SystemFD/Metatheory/SemSoundnessFail.lean
@@ -1,0 +1,564 @@
+import SystemFD.Term
+import SystemFD.Term.Subexpression
+import SystemFD.Term.Variant
+import SystemFD.Metatheory.Canonicity
+import SystemFD.Metatheory.Confluence
+import SystemFD.Metatheory.Progress
+import SystemFD.Metatheory.Preservation
+
+set_option maxHeartbeats 500000
+
+/-
+
+Goal
+----
+
+We want to have a syntactic property P on terms of SystemFD
+(possibly indexed over types and context)
+st. the following holds for it:
+
+   P τ t ⇒
+   ∃ n, (t ⟶⋆ n) ∧
+        (Val Γ n ∧ n is confusion free)
+        ∨ ( does not have a normal form)
+
+The context Γ has to bear some responsibility for the term to be confusion free,
+as the · ⟶⋆ · relation is dependent on Γ for instantiating open methods. We call this
+property saturation. Intuitively, the saturation property enforces that the
+(well typed) open method call instantiations cannot cause confusion.
+
+To explicitly encode this property in our formalization:
+
+   SatCtx Γ ∧ P τ Γ t ⇒
+   ∃ n, (t ⟨Γ⟩⟶⋆ n) ∧
+        (Val Γ n ∧ n is confusion free)
+         ∨ n does not have a normal form
+
+
+Confusion Free (or (Weakly) Determined):
+---------------
+
+Idea 1:
+
+Determined Γ τ t
+
+A (well typed) term, t,
+1. t does not contain `0 or ⊕ or guards (at the head)
+2. open methods are fine but they need to be fully applied -- enforced by typing?
+
+
+Idea 2:
+DeterminedTyping Γ t τ
+
+Deeply checked  Idea 1. check that t does not contain `0, ⊕ etc only at the head but for all subterms of t
+
+theorem : NoConfusion Γ → Closed Γ → DetermindedTyping Γ t τ
+          Val Γ t  ∨ (∃ t', t ⟶+ t' ∧ DetermindedTyping Γ t' τ)
+
+m [τs] ds : σ
+
+NoConfusion Γ
+
+    ∀ τs ds,
+      (τs are ground, ds are DeterminedTyping Γ σ d, σ is ground)
+    ∃ i, Γ d@ i = .inst #m t ∧ t [τs] ds - ̸⟶⋆ `0 ∧
+    ∀ k, k ≠ i ∧  Γ d@ k = .inst #m t' ∧ t' [τs] ds ⟶⋆ `0
+
+Captures: Saturation.
+1. Instance existence --> no `0
+2. Instance uniqueness --> no ⊕
+
+
+Equivalent to:
+∀ m [τs] ds : σ ⟶+ n, DeterminedTyping Γ n σ
+
+
+-/
+
+namespace Term
+
+def mk_ty_tm_app (t : Term) (τs : List Term) (es : List Term) := (t.mk_ty_apps τs).mk_apps es
+notation:70 t:170 "⬝[" τs:170 "]⬝" es:170 "⬝" => mk_ty_tm_app t τs es
+
+-- Ground Types are the ones that are not lambda bound
+-- Int, Bool, Int → Bool, Maybe, Maybe Int are all ground types
+-- a → Int, Maybe a are not ground types
+def groundTy (Γ : Ctx Term) : Term -> Bool
+| #x => Γ.is_datatype x || Γ.is_opent x
+| (τ1 -t> τ2) => groundTy Γ τ1 && groundTy (.empty :: Γ) τ2
+| τ1 `@k τ2 => groundTy Γ τ1 && groundTy  Γ τ2
+| _ => false
+
+end Term
+
+namespace Ctx
+
+end Ctx
+
+@[simp]
+abbrev Determined (Γ : Ctx Term) (t : Term) : Prop := ¬ contains_variant Γ.variants [.zero, .guard, .ctor2 .choice] t
+
+
+@[simp]
+abbrev Confused (Γ : Ctx Term) (t : Term) : Prop := contains_variant Γ.variants [.zero, .guard, .ctor2 .choice] t
+
+theorem partition_confusion_determined {Γ : Ctx Term}  {t : Term} : Determined Γ t <-> ¬ Confused Γ t :=
+ by simp
+
+
+@[simp]
+abbrev DeterminedWellTyped (Γ : Ctx Term) (τ t: Term) : Prop :=
+  Γ ⊢ t : τ ∧  Determined Γ t
+
+@[simp]
+abbrev DeterminedWellTypedVal (Γ : Ctx Term) (τ t: Term) : Prop :=
+  Γ ⊢ t : τ ∧  Determined Γ t ∧ Val Γ t
+
+-- TODO: Generalize this to mean also that open methods are fully applied
+
+
+namespace Ctx
+
+@[simp]
+-- A closed context is a context where there are only pure declarations and no let, lambda bound terms
+abbrev Closed (Γ : Ctx Term) : Prop :=
+  ⊢ Γ ∧  ∀ (x : Nat), Γ.is_stable_red x
+
+@[simp]
+abbrev Determined Γ := ∀ x, Γ.is_openm x ->
+  -- ∀ sp :  List (SpineVariant × Term), ∀ σ : Term,
+  ∀ τs ds : List Term, ∀ σ : Term,
+  σ.groundTy Γ ->
+  (Γ ⊢ ((#x) ⬝[τs]⬝ ds ⬝) : σ) -> -- TODO generalize this to arbitrary spine
+  -- (Γ ⊢ ((#x).apply_spine sp) : σ)
+  -- (∀ τ ∈ τs, τ.groundTy Γ) ->
+  (∀ d ∈ ds, ∃ κ, DeterminedWellTypedVal Γ κ d) ∧
+  ∃ n, ((#x) ⬝[τs]⬝ ds ⬝) ⟨Γ⟩⟶⋆ n ∧ DeterminedWellTyped Γ σ n
+
+@[simp]
+abbrev DeterminedClosedCtx Γ := Determined Γ ∧ Closed Γ
+end Ctx
+
+
+theorem closed_ctx_has_no_vars (Γ : Ctx Term) : Γ.DeterminedClosedCtx -> (∀ x, ¬ Γ.is_type x) := by
+ intro h; cases h; case _ h2 =>
+ simp at h2; cases h2; case _ h2 =>
+ intro x; replace h2 := h2 x; intro h3; unfold Ctx.is_type at h3;
+ replace h3 := type_indexing_exists h3; cases h3; case _ h3 =>
+ rw[h3] at h2; unfold Frame.is_stable_red at h2; simp at h2
+
+
+-- A direct proof of this lemma obviously fails
+theorem NoConfusionProgressFail Γ σ t:
+  Γ.Determined -> Γ.Closed -> DeterminedWellTyped Γ σ t ->
+  Val Γ t ∨
+  (∃ t', t ⟨Γ⟩⟶+ t' ∧ DeterminedWellTyped Γ σ t') := by
+intro h1 h2 h3
+have no_var := closed_ctx_has_no_vars Γ (by constructor; assumption; assumption)
+simp at h3; cases h3; case _ wt noc =>
+have lem_p := progress no_var wt
+cases lem_p
+case _ => constructor; assumption
+case _ lem_p =>
+  cases lem_p
+  case _ h =>
+    cases h; case _ t' r =>
+    apply Or.inr;
+    have lem_pres := preservation wt (RedStar.step RedStar.refl r)
+    have lem_prog := progress no_var lem_pres
+    cases lem_prog
+    case _ h =>
+      exists t'
+      constructor
+      · constructor; constructor; assumption
+      · sorry
+  -- Have : Γ ⊢ t ⟶ t' : σ. t' is value.
+  -- Show: t' has no confusion
+  -- we know that NoConfusionWellTyped property is not directly preserved over reduction relation
+    case _ h =>
+      cases h;
+      case _ h => sorry
+      case _ h => exfalso; sorry
+  case _ e => exfalso; rw[e] at noc; simp at noc
+
+
+-- Attempt 1: Generalize NoConfusion of terms indexed by its type
+-- This is very similar to the Strong Normalization Predicate (indexed by types) for terms
+
+inductive SemDetermined (Γ : Ctx Term) : Term -> Term -> Prop
+| AppTy :
+  Γ.DeterminedClosedCtx ->
+  τ = Term.mk_kind_apps #x τs ->
+  DeterminedWellTyped Γ τ t ->
+  (∃ t', t ⟨Γ⟩⟶+ t' ∧ DeterminedWellTyped Γ τ t') ->
+  SemDetermined Γ τ t
+| ArrowTy :
+  Γ.DeterminedClosedCtx ->
+  DeterminedWellTyped Γ (τ1 -t> τ2) f ->
+  ∀ e, SemDetermined Γ τ1 e ->
+  σ' = τ2 β[e] ->
+  SemDetermined Γ σ' (f `@ e)
+| AllTy :
+  Γ.DeterminedClosedCtx ->
+  DeterminedWellTyped Γ (∀[K] σ) f ->
+  ∀ τ, Γ ⊢ τ : K ->
+  σ' = σ β[τ] ->
+  SemDetermined Γ σ' (f `@t τ)
+| EqTy :
+  Γ.DeterminedClosedCtx ->
+  ∀ τ1 τ2, Γ ⊢ τ1 : K -> Γ ⊢ τ2 : K ->
+  (∃ t', t ⟨Γ⟩⟶+ t' ∧ DeterminedWellTyped Γ (τ1 ~[K]~ τ2) t') ->
+  SemDetermined Γ (τ1 ~[K]~ τ2) t
+
+
+theorem subst_determined_stable_lemma {Γ Δ : Ctx Term} {σ : Subst Term} {τ e}:
+  (∀ n : Nat, ∃ t, σ n = .su t -> ∃ τ, DeterminedWellTyped Γ τ t) ->
+
+  DeterminedWellTyped Γ τ e ->
+  DeterminedWellTyped Δ ([σ] τ) ([σ] e) := by
+intro h1 h2
+sorry
+
+
+
+-- Need to now show stability over substitutions
+theorem subst_determined_stable {Γ : Ctx Term} {τ τ' t e : Term} :
+  DeterminedWellTyped (.type τ' :: Γ) τ t ->
+  DeterminedWellTyped Γ τ' e ->
+  DeterminedWellTyped Γ (τ β[e]) (t β[e]) := by
+intro h1 h2
+apply @subst_determined_stable_lemma (Frame.type τ' :: Γ) Γ _ τ t
+case _ =>
+  intro n
+  induction n
+  exists e; intro h; exists τ;
+  sorry
+  sorry
+assumption
+
+
+theorem NoConfusionProgressFail2 :
+  SemDetermined Γ σ t ->
+  Val Γ t ∨
+  (∃ t', t ⟨Γ⟩⟶+ t' ∧ DeterminedWellTyped Γ σ t') := by
+intro h
+induction h
+case _ => apply Or.inr; assumption
+case _ ih =>
+  cases ih
+  case _ τ1 τ2 f _ _ j1 e j2 _ ih =>
+    simp at j1;
+    cases j1; case _ j1 _ =>
+    have no_var : ∀ x, ¬ Γ.is_type x := by apply closed_ctx_has_no_vars; assumption
+    have lem_prog := progress no_var j1
+    cases lem_prog;
+    case _ h =>
+      have f_shape := canonical_lambda j1; simp at f_shape;
+      replace f_shape := f_shape h j1;
+      have lem := classification_lemma j1; simp at j1; cases lem;
+      case _ h => cases h
+      case _ h =>
+        cases h;
+        case _ h => have lem := classification_lemma h; cases h
+        case _ h => cases h; case _ h => cases h; case _ h =>
+          have lem := invert_arr_kind h; cases lem;
+          replace f_shape := f_shape h
+          have lem : ArrowLike (τ1 -t> τ2) := by constructor
+          replace f_shape := f_shape lem;
+          induction f_shape
+          case _ τ t _ =>
+            apply Or.inr
+            have lem : τ = τ1 := lam_typing_unique2 j1; cases lem
+            exists (t β[e])  --> needs substitution is stable over NoConfusion
+            constructor
+            sorry
+            sorry
+
+          case _ => /- illtyped (Λ[k] f `@ t) -/ cases j1
+          case _ vh _ => /- (ctor `@ e) is a value -/
+            apply Or.inl;
+            cases vh; case _ t _ _ nf =>
+              cases nf; case _ w nf ctor =>
+              constructor
+              have lem := Term.neutral_form_law nf
+              rw[<-lem]; simp; rw[Option.bind_eq_some];
+              exists w; simp;
+              constructor;
+              rw[lem]; apply Eq.symm nf
+              constructor; exact rfl; exact rfl
+              simp at ctor;  apply Frame.is_ctor_implies_is_stable_red ctor
+          case _ vh _ => /- inst `@ e -/
+            apply Or.inl;
+            cases vh; case _ t _ _ nf =>
+              cases nf; case _ w nf inst =>
+              constructor
+              have lem := Term.neutral_form_law nf
+              rw[<-lem]; simp; rw[Option.bind_eq_some];
+              exists w; simp;
+              constructor;
+              rw[lem]; apply Eq.symm nf
+              constructor; exact rfl; exact rfl
+              simp at inst;  apply Frame.is_insttype_implies_is_stable_red inst
+
+          case _ => simp at * --> contradiction
+    case _ h =>
+      cases h
+      case _ h =>
+
+        sorry
+      case _ h => exfalso; cases h; simp at *
+  case _ ih =>
+    cases ih; case _ f _ _ _ _ _ _ e' ih =>
+    cases ih;
+    apply Or.inr; exists (f `@ e');
+    constructor;
+    case _ h1 _ _ _ _ h2 =>
+      simp at h1; cases h1;
+      simp at h2; cases h2;
+      case _ j1 _ j2 _ =>
+      sorry
+    -- sorry
+    simp; constructor
+    · sorry -- -t> bullshit
+    · constructor;
+      case _ h _ _ _ _ _ => simp at h; cases h; assumption
+      case _ h => simp at h; cases h; assumption
+
+case _ => sorry
+case _ => apply Or.inr; assumption
+
+
+-- Determined needs to be defined using a recursive function.
+-- But we cannot because substitutions get in the way
+def SemDetermined' (Γ : Ctx Term) : Term -> (Term -> Prop)
+| τ1 -t> τ2 => λ f =>
+  Γ.DeterminedClosedCtx ->
+  DeterminedWellTyped Γ (τ1 -t> τ2) f ->
+  ∀ e, SemDetermined' Γ τ1 e ->
+  -- σ' = τ2 β[e] ->
+  SemDetermined' Γ (τ2 β[e]) (f `@ e)
+| ∀[K] σ => λ f =>
+  Γ.DeterminedClosedCtx ->
+  DeterminedWellTyped Γ (∀[K] σ) f ->
+  ∀ τ, Γ ⊢ τ : K ->
+  -- σ' = σ β[τ] ->
+  SemDetermined' Γ (σ β[τ]) (f `@t τ)
+| (τ1 ~[K]~ τ2) => λ t => -- in this case t should just step to refl
+  Γ.DeterminedClosedCtx ->
+  Γ ⊢ τ1 : K -> Γ ⊢ τ2 : K ->
+  (∃ t', t ⟨Γ⟩⟶+ t' ∧ DeterminedWellTyped Γ (τ1 ~[K]~ τ2) t') ->
+  SemDetermined' Γ (τ1 ~[K]~ τ2) t
+| τ => λ t =>
+  Γ.DeterminedClosedCtx ->
+  ∃ x τs, τ = Term.mk_kind_apps #x τs ->
+  DeterminedWellTyped Γ τ t ->
+  (∃ t', t ⟨Γ⟩⟶+ t' ∧ DeterminedWellTyped Γ τ t') ->
+  SemDetermined' Γ τ t
+-- termination_by λ τ t =>  sorry
+decreasing_by
+  case _ => unfold sizeOf; unfold sizeOf_Term; simp; omega
+  case _ => sorry
+  case _ => sorry
+  case _ => sorry
+  case _ => sorry
+
+
+/-
+
+is confusion free if for all term contexts C[⬝], and saturated context Γ
+C[t] ⟨Γ⟩ ⟶⋆ n s.t. n is a value and n does not contain open methods or `0 or ⊕ or guards
+
+Its definitely not the case that any C[⬝] would do.  Why?
+C[⬝] itself can easily induce confusion:
+if C[⬝] = 3 ⊕ ⬝ then any confusion free term results in confusion
+
+Idea:
+Apply some restriction on C[⬝].
+A term context C[⬝] is confusion free if it does not contain open methods, `0, ⊕ or guards
+The key observation is that confusion can be induced by only these 4 constructs.
+
+
+Take 2: A term is confusion free if in any confusion free term context  C[⬝], and a saturated context Γ
+C[t] ⟨Γ⟩ ⟶⋆ n s.t. n is a value (or it loops indefinitely) and n does not
+contain open methods or `0 or ⊕ or guards
+
+
+Maybe what we need is a measure for confusion for term contexts.
+
+
+
+
+
+
+Context Saturation:
+-------------------
+Intuitively, a context Γ is saturated
+If for any open method in the context, there is only one instance that does not make the term vanish.
+
+Suppose `m` is the open method. with type ∀ τs. Qs ⇒ τ'
+now, consider all possible (well typed applications) of this open method.
+WLOG, `m [τs] ds` such that Γ ⊢ d : Q[α ↦ τ], Γ ⊢ m [τs] ds : τ'[α ↦ τ]
+
+now, `m` will have some associated instantiations I_j in the context of the form (Λ αs .guards ... )
+so `m [τs] ds` ⟶ (I_1 ⊕ I_2 ⊕ .. I_n) [τs] ds ⟶⋆ (I_1 [τs] ds) ⊕ (I_2 [τs] ds) ⊕ ... ⊕ (I_n [τs] ds)
+
+Now we want saturation property to capture the idea only one of these I_j survives.
+
+Take 1:
+
+    ∀ τs ds,
+      (τs are ground, ds are confusion free)
+    ∃ i, Γ d@ i = .inst #m t ∧ t [τs] ds - ̸⟶⋆ `0 ∧
+    ∀ k, k ≠ i ∧  Γ d@ k = .inst #m t' ∧ t' [τs] ds ⟶⋆ `0
+
+but our saturation property is too strict! ds shouldn't be confusion free, they can
+very well contain calls to open methods. This is where related inputs go to related outputs
+idea gets used (I think). ds should satisfy the original goal property P from above.
+
+Option: Let P be collection of terms that contains no guards, `0, ⊕. (open methods are okay)
+This seems to have some merit. It is a syntactic check and with context saturation ensuring no confusion
+
+Take 2:
+
+    ∀ τs ds,
+      (τs are ground, ds satisfy property P)
+    ∃ i, Γ d@ i = .inst #m t ∧ t [τs] ds - ̸⟶⋆ `0 ∧
+    ∀ k, k ≠ i,  Γ d@ k = .inst #m t' → (t' [τs] ds ⟶⋆ `0)
+
+-/
+
+
+
+namespace TermCtx
+
+
+end TermCtx
+
+
+-- shallowly confusion free is a term that does not have a `0 or ⊕ at its head
+@[simp]
+abbrev ShallowlyConfusionFree (Γ : Ctx Term) : Term -> Prop
+| .zero => false
+| .ctor2 .choice _ _ => false
+| t => Term.isTerm Γ t
+
+
+-- Shalowly confusion free value is a value which also shallowly confusion free
+--   So, (λ x. `0) is a shallowly confusion free value.
+--   but  (`0  ⊕ `0) is not a shallowly confusion free value.
+@[simp]
+abbrev SCFVal (Γ : Ctx Term) (t: Term) := Val Γ t ∧ ShallowlyConfusionFree Γ t
+
+@[simp]
+abbrev CanCauseConfusion (Γ : Ctx Term) (t: Term) : Bool :=
+  Term.isTerm Γ t ∧
+  contains_variant Γ.variants [.var .openm, .zero, .guard, .ctor2 .choice] t
+
+
+-- a. Semantically,
+--    x is saturated iff
+--    ∀ τ e, x is open in Γ ->
+--    Val Γ e ->
+--    x[τ]e is of ground type ->
+--    (∃ v, x[τ]e ⟶★ v ∧ Shallowly Confusion Free Γ v)
+@[simp]
+abbrev Sat (Wf : Ctx Term -> Term -> Prop)(Γ : Ctx Term) (x : Nat):  Prop :=
+  ⊢ Γ ∧
+  Γ.is_openm x ->
+  (∀ τs es σ,
+      (∀ τ ∈ τs, τ.groundTy Γ) ->
+      (∀ e ∈ es, Wf Γ e) ->
+      (Γ ⊢ (#x ⬝[ τs ]⬝ es ⬝) : σ ∧ σ.groundTy Γ ∧ ∃ k, Γ ⊢ σ : k ∧ Γ ⊢ k : □) ->
+      (∃ v, (#x ⬝[ τs ]⬝ es ⬝) ⟨ Γ ⟩⟶⋆ v ∧ Wf Γ v))
+
+@[simp]
+-- if the variable is not an open thingy then it is automatically saturated
+abbrev SatCtx (Wf : Ctx Term -> Term -> Prop) (Γ : Ctx Term) : Prop := ∀ x, Γ.is_openm x -> Sat Wf Γ x
+
+-- Question: Is the term (λ x. `0) a value, but applying it to anything will make it vanish
+-- Weak Determinism is how we handle open methods
+-- this is where guards come in.
+-- in any context evaluation C, t is weakly deterministic
+-- if C[t] -->* doesn't reduce to `0 or ⊕ i.e. it is shallowly deterministic value.
+
+-- "Shallowness": Terms that we know reduce to `0 (or not) in "one step"
+-- Reductions do not preserve shallowness
+
+-- Semantic Characterization of a Weakly Deterministic Value
+@[simp]
+abbrev CFVal (Wf : Term -> Prop) (t : Term): Prop := ∀ Γ,
+    -- ¬ (ContainsVariant (Ctx.variants Γ) [.zero, .guard, .ctor2 .choice] t) ∧
+    -- Complaint: this is syntactic not semantic
+    -- (∀ x : Nat, Term.Subexpr #x t -> Γ.is_openm x -> (SemSat P Γ #x)) ->
+    -- (∃ v, t ⟨ Γ ⟩⟶⋆ v ∧ CFVal Wf Γ v) ->
+    Γ.Closed ->
+    SatCtx ShallowlyConfusionFree Γ ->
+    Val Γ t ->
+    Wf t
+
+
+inductive CFTerm (Wf : Term -> Prop) (Γ : Ctx Term) : Term -> Prop where
+| WDBase :
+    Wf M ->
+    CFTerm Wf Γ M
+| WDChoice1 :
+   CFTerm Wf Γ M ->
+   (N ⟨ Γ ⟩⟶⋆ `0) ->
+   CFTerm Wf Γ (M ⊕ N)
+| WDChoice2 :
+   CFTerm Wf Γ N ->
+   (M ⟨ Γ ⟩⟶⋆ `0) ->
+   CFTerm Wf Γ (M ⊕ N)
+
+-- chain
+theorem sanity :
+  CFTerm (λ M => ∃ v, (M ⟨ Γ ⟩⟶⋆ v) ∧ Val Γ v) Γ M ->
+  ∃ v, (M ⟨ Γ ⟩⟶⋆ v) ∧ Val Γ v := by
+intro h;
+induction h
+assumption
+case _ M N h1 h2 ih =>
+  cases ih; case _ v ih =>
+  cases ih; case _ ih1 ih2 =>
+  have lem : (M ⊕ N) ⟨ Γ ⟩⟶⋆ (v ⊕ `0) := by
+    apply reds_choice_parallel ih1 h2
+  have lem2 : (v ⊕ `0) ⟨ Γ ⟩⟶⋆ v := by apply RedStar.step; (apply RedStar.refl); constructor
+  exists v
+  constructor
+  apply reds_trans lem lem2
+  assumption
+
+case _ N M h1 h2 ih =>
+  cases ih; case _ v ih =>
+  cases ih; case _ ih1 ih2 =>
+  have lem : (M ⊕ N) ⟨ Γ ⟩⟶⋆ (`0 ⊕ v) := by
+    apply reds_choice_parallel h2 ih1
+  have lem2 : (`0 ⊕ v) ⟨ Γ ⟩⟶⋆ v := by apply RedStar.step; (apply RedStar.refl); constructor
+  exists v
+  constructor
+  apply reds_trans lem lem2
+  assumption
+
+-- Next step:
+-- 1. What does saturation mean?
+-- a. Semantically
+--    x is saturated iff
+--    ∀ τ e, x is open in Γ ->
+--    WDVal Γ e ->
+--    x[τ]e is of ground type ->
+--    x[τ]e -->* ∃ v. WDVal Γ v
+
+-- b. Syntactically
+--    AI: We don't have a syntactic characterization yet, maybe we never need it for our purposes.
+--    After all, when a programmer uses an overloaded operator, there is no indication that
+--    that function will actually be fine at runtime syntactically. It is only when the typechecker
+--    works on it (does some typed semantic analysis) is when it can generate an instance to fill in
+--    that decides what the behavior of the overloaded function is. Open term variables in our case
+--    _are_ the  overloaded functions
+
+-- c. Syntactic saturation => semantic saturation
+
+
+-- 2. Syntactic Weakly deterministic Term => Semantic Weakly Deterministic Term
+-- Way 1: Syntactic WD Term to use Semantic saturation
+-- And then try proving 2.
